---
title: "Using the rearranging equations: answers"
author: "Shanelle Advani, Ciara Cormican"
abstract-title: Summary
abstract: The answers to a selection of questions for the study guide on introduction to rearranging equations.

---

*These are the answers to [Questions: Introduction to rearranging equations](qs-introtorearrange.qmd).* **Please attempt the questions before reading these answers!**

## Questions {-}

### 1 {-}

For each of the equations below, rearrange the equation so that ğ‘¥ is the subject of the equation.

1.1 $x^2 âˆ’ 12ğ‘ = 11ğ‘ + 6b^2$.
$$x^2 = 12ğ‘ + 11ğ‘ + 6b^2$$
$$\sqrt{x^2} = \sqrt{23a + 6b^2}$$
$$x = \pm\sqrt{23a + 6b^2}$$

1.2. $y^2 + 14x = 8x + 10z$.
$$y^2 + 14x - 8x = 10z$$
$$6x = 10z - y^2$$
$$x = \frac{5}{3}z - \frac{1}{6}y^2$$

1.3. $h^4 âˆ’ x^3h = âˆ’56h^4$.
$$h(h^3 âˆ’ x^3) = âˆ’56h^4$$
$$h^3 âˆ’ x^3 = âˆ’56h^3$$
$$h^3 + 56h^3 = x^3$$
$$x^3 = 57h^3$$
$$\sqrt[3]{x^3} = \sqrt[3]{57h^3}$$
$$x = \sqrt[3]{57}h$$

1.4. $x^4 = y^2$
$$\sqrt[4]{x^4} = \sqrt[4]{y^2}$$
$$x = \pm\sqrt{y}$$


### 2 {-}

Make T the subject of the equation

2.1 $\frac{L}{g} = (\frac{T}{2\pi})^2$.
$$\pm\sqrt{\frac{L}{g}} = \sqrt{(\frac{T}{2\pi})^2}$$
$$\frac{T}{2\pi} = \pm\sqrt{\frac{L}{g}}$$
$$T = \pm 2\pi\sqrt{\frac{L}{g}}$$
2.2. $h^2 = T^2 + b^2$.
$$T^2 = h^2 - b^2$$
$$\sqrt{T^2} = \pm \sqrt{h^2 - b^2}$$
$$T = \sqrt{h^2 - b^2}$$


### 3 {-}

For each of the equations below, rearrange the equation so that ğ‘¥ is the subject of the equation.

1.1. $v^2 = x^2 + 2as$
$$v^2 - 2as = x^2$$
$$\sqrt{x^2} = \sqrt{v^2 - 2as}$$
$$x = \pm\sqrt{v^2 - 2as}$$
1.2. $8y + \sqrt[3]{xy} + 14 = 10z$
$$\sqrt[3]{xy}= 10z - 8y- 14$$
$$(\sqrt[3]{xy})^3= (10z - 8y- 14)^3$$
$$xy= (10z - 8y- 14)^3$$
$$x= y(10z - 8y- 14)^3$$

1.3. $8 x^{1.5} = \sqrt[3]{x}$
$$(8 x^{1.5})^3 = (\sqrt[3]{x})^3$$

$$8^3 x^{4.5} = x$$


$$512 x^{3.5} = 1$$
$$x^{3.5} = \frac{1}{512}$$
$$\sqrt[3.5]{x^{3.5}} = \sqrt[3.5]{\frac{1}{512}}$$
$$x = \frac{1}{\sqrt[3.5]{512}}$$


1.4. $y^2 + 2y + \sqrt[5]{x} = 4$
$$ \sqrt[5]{x} = 4 - y^2 - 2y $$
$$ (\sqrt[5]{x})^5 = (4 - y^2 - 2y)^5 $$
$$ x = (4 - y^2 - 2y)^5 $$



