---
title: "Vector addition and scalar multiplication"
author: "Renee Knapp, Kin Wang Pang"
abstract-title: Summary
abstract: Understanding and utilising vector addition and scalar multiplication are essential when studying vectors, particularly when it comes to solving equations involving vectors.
categories:
  - Geometry
  - Vectors
  - Linear mathematics
image: FiguresPNG/addandsm-image.png
---

```{r, setup, include = FALSE}
library("webexercises")
```

*Before reading this guide, it is recommended that you read [Guide:
Introduction to vectors](introductiontovectors.qmd).*

<!--Besides the 3 Figures (6 links to total), there are 3 hyperlinks to other .qmd files: line 93,343,347-->

# What is vector addition and scalar multiplication? {-}

As you have seen in [Guide: Introdution to vectors](introductiontovectors.qmd), vectors have a magnitude and a direction and are represented in coordinate spaces by components, either in $\mathbf{i},\mathbf{j},\mathbf{k}$ notation or as a column vector. These components can be considered independent to each other. 

You are able to add two vectors together, or multiply a vector by a scalar. To do this, you have to consider each component of the vector individually. These ideas of vector addition and scalar multiplication are key concepts in **linear mathematics**, which underpins many important concepts in applied mathematics, physics, chemistry, statistics, economics, and computer science -- linear mathematics is even used in generative AI and machine learning!

This guide introduces vector addition and scalar multiplication, for vectors in both $\mathbf{i}$,$\mathbf{j}$,$\mathbf{k}$ and column notation, and explains the role of vector addition and scalar multiplication in solving equations using vectors.

Following the lead of [Guide: Introduction to vectors](introductiontovectors.qmd) this guide solely works on vectors in **three dimensions**.

# Vector addition and subtraction {-}

## Definition and initial examples {-}

The addition of vectors $\mathbf{u}$ and $\mathbf{v}$ is defined by following $\mathbf{u}$ and then $\mathbf{v}$. More specifically, you can join the start of a vector $\mathbf{v}$ to the end of another vector $\mathbf{u}$, and then draw a vector $\mathbf{u}+\mathbf{v}$ from the start of $\mathbf{u}$ to the end of $\mathbf{v}$. See Figure @fig-1 for a picture of this process.

::: {.content-visible when-format="html"}

![Graphical representation of vector addition. The three steps of the process are labelled.](./FiguresPNG/17-1.png){#fig-1
width="100%" fig-alt="(1) There are two vectors u and v. (2) The head of vector u is joined to the tail of vector v. (3) This forms a triangle and the new vector u + v is created by completing the triangle. This vector points from the tail of u to the head of v."}

::: 

::: {.content-hidden when-format="html"}
![Graphical representation of vector addition. The three steps are labelled.](./FiguresPNG/17-1.png){#fig-1
width="100%" fig-alt="(1) There are two vectors u and v. (2) The head of vector u is joined to the tail of vector v. (3) This forms a triangle and the new vector u + v is created by completing the triangle. This vector points from the tail of u to the head of v."}

::: 

What does this mean for a vector written in $\mathbf{i},\mathbf{j},\mathbf{k}$ notation? Examining the $\mathbf{i}$ component of the vector $\mathbf{u}+\mathbf{v}$, you can notice that you first move using $\mathbf{i}$ component of $\mathbf{u}$ and then move by the $\mathbf{i}$ component of $\mathbf{v}$. It follows that the $\mathbf{i}$ component of the vector $\mathbf{u}+\mathbf{v}$ is the sum of the $\mathbf{i}$ component of $\mathbf{u}$ and $\mathbf{i}$ component of $\mathbf{v}$. You can expand this to both the $\mathbf{j}$ and $\mathbf{k}$ components of $\mathbf{u}+\mathbf{v}$ to get the following definition. 

::: callout-note
## Definition of vector addition

Let $\mathbf{a} = a_1 \mathbf{i} + a_2 \mathbf{j} + a_3 \mathbf{k}$ and
$\mathbf{b} = b_1 \mathbf{i} + b_2 \mathbf{j} + b_3 \mathbf{k}$ be two vectors. Then the **addition of the two vectors**, written as $\mathbf{a} + \mathbf{b}$, is defined as follows:
$$\mathbf{a} + \mathbf{b} = (a_1+b_1) \mathbf{i} + (a_2 + b_2) \mathbf{j} + (a_3 + b_3)\mathbf{k}.$$
In column vector notation, the addition of $\mathbf{a} = \begin{bmatrix}a_1\\a_2\\a_3\end{bmatrix}$ and
$\mathbf{b} = \begin{bmatrix}b_1\\b_2\\b_3\end{bmatrix}$ is: 
$$\mathbf{a} + \mathbf{b} = \begin{bmatrix}a_1 + b_1\\a_2 + b_2\\a_3 + b_3\end{bmatrix}.$$

:::

::: {.callout-note appearance="simple"}
## Example 1

You are given $\mathbf{a} = 3\mathbf{i} + 4\mathbf{j} - 8\mathbf{k}$ and
$\mathbf{b} = 2\mathbf{i} +8\mathbf{j} + 12\mathbf{k}$. Then
\begin{align*}
\mathbf{a} + \mathbf{b} &= (3\mathbf{i} + 4\mathbf{j} - 8\mathbf{k}) + (2\mathbf{i} +8\mathbf{j} + 12\mathbf{k})\\
&=(3+2)\mathbf{i} + (4+8)\mathbf{j} + (-8 + 12)\mathbf{k}\\
&=5\mathbf{i} + 12\mathbf{j} + 4\mathbf{k}
\end{align*}

:::

::: {.callout-note appearance="simple"}
## Example 2

You are given $\mathbf{a} = \begin{bmatrix}3\\4\\-2\end{bmatrix}$ and $\mathbf{b} = \begin{bmatrix}5\\6\\14\end{bmatrix}$.
Then $$\mathbf{a} + \mathbf{b} = \begin{bmatrix}3\\4\\-2\end{bmatrix} + \begin{bmatrix}5\\6\\14\end{bmatrix} = \begin{bmatrix}3+5\\4+6\\-2 + 14\end{bmatrix} = \begin{bmatrix}8\\10\\12\end{bmatrix}.$$

:::

<!-- In the above diagram, the two vectors $\mathbf{u}$ and $\mathbf{v}$ are shown. The addition of the two vectors is the process of joining the head of one of the vectors to the tail of another. Then completing the triangle to form the new vector. -->

To *subtract* one vector from another, you can use the definition of a negative vector from [Guide: Introduction to vectors](introductiontovectors.qmd). Much like for numbers, you can write that $$\mathbf{u} - \mathbf{v} = \mathbf{u} + (-\mathbf{v}).$$ So to subtract to vectors, you need to add $-\mathbf{v}$ to $\mathbf{u}$ using vector addition.

Geometrically, you need tp reverse the direction of the vector $\mathbf{v}$ first before finding $\mathbf{u} + (-\mathbf{v})$ in the usual fashion. @fig-2 explains this process.

::: {.content-visible when-format="html"}
![Graphical representation of vector subtraction. The four steps are labelled.](./FiguresPNG/18-2.png){#fig-2
width="100%" fig-alt="(1) There are two vectors u and v. (2) The direction of vector v is reversed in direction to form the negative v vector. (3) Then the head of vector u joins the tail of vector -v. (4) Completing the triangle gives the vector u - v. This vector points from the tail of u to the head of -v."}

::: 

::: {.content-hidden when-format="html"}
![Graphical representation of vector subtraction](./FiguresPNG/18-2.png){#fig-2
width="100%" fig-alt="(1) There are two vectors u and v. (2) The direction of vector v is reversed in direction to form the negative v vector. (3) Then the head of vector u joins the tail of vector -v. (4) Completing the triangle gives the vector u - v. This vector points from the tail of u to the head of -v."}

::: 

::: {.callout-note appearance="simple"}
## Example 3

You are given $\mathbf{a} = 3\mathbf{i} + 4\mathbf{j} + 3\mathbf{k}$ and
$\mathbf{b} = 5\mathbf{i} - 6\mathbf{j}$. Then
\begin{align*}
\mathbf{a} - \mathbf{b} &= \mathbf{a} + (-\mathbf{b})\\
&= (3\mathbf{i} + 4\mathbf{j} + 3\mathbf{k}) + (-5\mathbf{i} + 6\mathbf{j})\\
&= (3-5)\mathbf{i} + (4+6)\mathbf{j} + (3 + 0)\mathbf{k}\\
&= -2\mathbf{i} + 10\mathbf{j} + 3\mathbf{k}
\end{align*}
:::

You can notice that you don't need to work out $-\mathbf{b}$ or similar; notice that if $\mathbf{a} = a_1 \mathbf{i} + a_2 \mathbf{j} + a_3 \mathbf{k}$ and
$\mathbf{b} = b_1 \mathbf{i} + b_2 \mathbf{j} + b_3 \mathbf{k}$, then
$$\mathbf{a} - \mathbf{b} = (a_1-b_1) \mathbf{i} + (a_2 - b_2) \mathbf{j} + (a_3 - b_3)\mathbf{k}$$ or, in column notation, $$\mathbf{a} - \mathbf{b} = \begin{bmatrix}a_1 - b_1\\a_2 - b_2\\a_3 - b_3\end{bmatrix}.$$

:::{.callout-warning}
Be careful with your signs when subtracting vectors in this way!
:::

::: {.callout-note appearance="simple"}
## Example 4

You are given $\mathbf{a} = \begin{bmatrix}3\\0\\-2\end{bmatrix}$ and $\mathbf{b} = \begin{bmatrix}5\\6\\-14\end{bmatrix}$.
Then $$\mathbf{a} - \mathbf{b} = \begin{bmatrix}3\\0\\-2\end{bmatrix} - \begin{bmatrix}5\\6\\-14\end{bmatrix} = \begin{bmatrix}3-5\\0-6\\-2 - (-14)\end{bmatrix} = \begin{bmatrix}-2\\-6\\12\end{bmatrix}.$$
:::


<!-- You may realize that vector addition is scalar addition done in a component manner, that is you sum of the magnitude of the $\textbf{i}$th component, the $\textbf{j}$th component and the $\textbf{k}$th component independently. -->
<!-- Thus vector addition inherits properties from scalar addition as well. -->

## Properties of vector addition

The process of adding vectors via their components is called **componentwise addition**. The addition of the components is the same as adding numbers, so you may expect properties of adding numbers to be reflected in vector addition. In fact, the following properties are true for **all** vectors $\mathbf{u},\mathbf{v},\mathbf{w}$.

-   $\mathbf{u} + \mathbf{v} = \mathbf{v} + \mathbf{u}$ (called **commutativity**)

-   $(\mathbf{u} + \mathbf{v}) + \mathbf{w} = \mathbf{u} + (\mathbf{v} + \mathbf{w})$ (called **associativity**).

The **zero vector** (see [Guide: Introduction to vectors](introductiontovectors.qmd)) plays an important role in properties of vector addition. In fact, there are two more properties relating entirely to the zero vector, which are true for all vectors $\mathbf{u}$:

-   $\mathbf{0} + \mathbf{u} = \mathbf{u}$

-   $\mathbf{u} + (-\mathbf{u}) = \mathbf{0}$

::: {.callout-note appearance="simple"}
## Example 5

You are given $\mathbf{a}= 2\mathbf{i}+ y\mathbf{j}-3\mathbf{k}$. Then $$\mathbf{a} + \mathbf{0} = (2+0)\mathbf{i}+ (y+0)\mathbf{j}+(-3+0)\mathbf{k} = 2\mathbf{i}+ y\mathbf{j}-3\mathbf{k} = \mathbf{a}$$ (as you would expect!)
:::

<!-- ::: {.callout-warning} -->

<!-- As vector addition is similar to scalar addition, then the rules for -->
<!-- expanding brackets follow. -->

<!-- $\mathbf{u} - \mathbf{v} + \mathbf{w} \neq\mathbf{u} - (\mathbf{v} + \mathbf{w})$ -->

<!-- ::: -->

<!-- ## The Zero vector -->

<!-- The zero vector $\mathbf{0}$ is defined as a vector with zero length. This -->
<!-- is different from the 0 scalar. You can learn more about the zero vector in [Guide: Introduction to Vectors](introductiontovectors.qmd) -->

<!-- The zero vector has the following properties: -->

::: {.callout-note appearance="simple"}
## Example 6

You are given $\mathbf{a} = \begin{bmatrix}2\\1\\0\end{bmatrix}$,
$\mathbf{b} = \begin{bmatrix}7\\2\\1\end{bmatrix}$ and $\mathbf{c} = \begin{bmatrix}-3\\-2\\5\end{bmatrix}.$ 

Then $\mathbf{a} + \mathbf{b} - \mathbf{c} = \begin{bmatrix}2+7 - (-3)\\1+2-(-2)\\0 + 1 - 5\end{bmatrix} = \begin{bmatrix}12\\5\\-4\end{bmatrix}$
:::

# Scalar multiplication {-}

## Definition and initial examples {-}

As was mentioned in [Guide: Introduction to vectors](introductiontovectors.qmd), another thing that you can do with vectors is to multiply it with a **scalar**, which is usually a real number. **Scalar multiplying** a vector by a positive scalar typically changes the magnitude of the vector and preserves the direction, and multiplying a vector by a negative scalar typically changes the magnitude of the vector and *reverses* the direction. @fig-3 shows a picture of these scenarios.

::: {.content-visible when-format="html"}
![Graphical representation of scalar multiplication.](./FiguresPNG/vectoradditionandscalarmultiplication-fig3.png){#fig-3
width="100%" fig-alt="There are five vectors side by side. Going from left to right, the first shows the general vector u. The second shows the vector lambda u, where lambda is larger than one. The vector is lambda times longer than the vector u, pointing in the same direction. The third vector shows the vector lambda u, where lambda is between one and zero. The magnitude of the vector is shorter than the original vector u by a factor of 1/lambda. The fourth vector shows lambda u, where lambda is between negative one and zero. The magnitude of the vector is shorter than the original vector u by a factor of 1/lambda, and the direction of the vector is reversed. The fifth vector shows the vector lambda u, where lambda is smaller than negative one. The magnitude of the vector is longer than the original vector u by a factor of lambda, and direction of the vector is inverted."}
:::

::: {.content-hidden when-format="html"}
![Graphical representation of scalar multiplication](./FiguresPNG/vectoradditionandscalarmultiplication-fig3.png){#fig-3
width="100%" fig-alt="There are five vectors side by side. Going from left to right, the first shows the general vector u. The second shows the vector lambda u, where lambda is larger than one. The vector is lambda times longer than the vector u, pointing in the same direction. The third vector shows the vector lambda u, where lambda is between one and zero. The magnitude of the vector is shorter than the original vector u by a factor of 1/lambda. The fourth vector shows lambda u, where lambda is between negative one and zero. The magnitude of the vector is shorter than the original vector u by a factor of 1/lambda, and the direction of the vector is reversed. The fifth vector shows the vector lambda u, where lambda is smaller than negative one. The magnitude of the vector is longer than the original vector u by a factor of lambda, and direction of the vector is inverted."}
:::


What does scalar multiplication do to the components of a vector? Suppose that you are scalar multiplying the vector $\mathbf{i}$. This is a unit vector, so has magnitude $1$. Since scalar multiplication by a scalar $\lambda$ (pronounced 'lambda') changes the length of a vector, it follows that the vector $\lambda\mathbf{i}$ has magnitude $|\lambda|$, the absolute value of $\lambda$. 

Since every vector $\mathbf{u}$ is the sum of scalar multiples of $\mathbf{i},\mathbf{j},\mathbf{k}$, it follows that $\lambda\mathbf{u}$ is the sum of scalar multiples of $\lambda\mathbf{i},\lambda\mathbf{j},\lambda\mathbf{k}$. This forms the basis of the definition:

<!-- You can represent scalar multiplication graphically. For different real scalars, the magnitude is multiplied by that amount. Note that if the scalar is negative, the direction of the vector is reversed. -->

::: callout-note
## Definition of scalar multiplication

Let $\mathbf{a} = a_1\mathbf{i} + a_2\mathbf{j} + a_3\mathbf{k}$ be a vector and let $\lambda$ be a real number. Then the **scalar multiple of $\mathbf{a}$ by $\lambda$** is given by $$\lambda \mathbf{a} = \lambda a_1\mathbf{i} + \lambda a_2\mathbf{j} + \lambda a_3\mathbf{k}.$$

In column notation, if $\mathbf{a} = \begin{bmatrix}a_1\\a_2\\a_3\end{bmatrix}$, then
$\lambda \mathbf{a} = \begin{bmatrix}\lambda a_1\\ \lambda a_2\\ \lambda a_3 \end{bmatrix}.$
:::

::: {.callout-note appearance="simple"}
## Example 7

You are given $\mathbf{a} = \begin{bmatrix}3\\5\\6\end{bmatrix}$. Then $5\mathbf{a} = \begin{bmatrix}5(3)\\5(5)\\5(6)\end{bmatrix} = \begin{bmatrix}15\\25\\30\end{bmatrix}.$
:::

::: {.callout-note appearance="simple"}
## Example 8

You are given $\mathbf{b} = -2\mathbf{i} + 6\mathbf{j} - 7\mathbf{k}$. Then
$$-3\mathbf{b} = (-3)(-2)\mathbf{i} + (-3)6\mathbf{j} - (-3)7\mathbf{k} = 6\mathbf{i} -18\mathbf{j} + 21\mathbf{k}.$$
:::


## Properties of scalar multiplication

Since scalar multiplication is similar to component-wise multiplication, then
it has the following properties for all vectors $\mathbf{u}$ and $\mathbf{v}$ and scalars $\lambda$ and $\mu$:

-   $(\lambda \mu) \mathbf{u} = \lambda (\mu \mathbf{u})$ (called **associativity of scalar multiplication**)

-   $( \lambda + \mu ) \mathbf{u} = \lambda \mathbf{u} + \mu \mathbf{u}$ (called **distributivity of scalar multiplication**)

-   $\lambda (\mathbf{u} + \mathbf{v}) = \lambda\mathbf{u} + \lambda\mathbf{v}$ (called **distributivity of vector addition**)

-   $1\mathbf{u} = \mathbf{u}$ (so $1$ is the **scalar multiplicative identity**)

In addition, the following are also true:

-   $0\mathbf{u} = \mathbf{0}$, so any vector scalar multiplied by $0$ gives the zero vector $\mathbf{0}$. 

-   $(-1)\mathbf{u} = -\mathbf{u}$

Finally, if two vectors are scalar multiples of each other, then they must have either the same direction or exactly opposite directions.

::: {.callout-tip}
If $\mathbf{u}$ and $\mathbf{v}$ are general vectors such that $\mathbf{u} = \lambda \mathbf{v}$ for some *positive* scalar $\lambda$, then $\mathbf{u}$ and $\mathbf{v}$ are **parallel** to each other. If $\mathbf{u} = \lambda \mathbf{v}$ for some *negative* scalar $\lambda$, then $\mathbf{u}$ and $\mathbf{v}$ are **antiparallel** to each other.

Equivalently, two vectors $\mathbf{u}$ and $\mathbf{v}$ are parallel if their correpsonding unit vectors are equal; so when $\hat{\mathbf{u}} = \hat{\mathbf{v}}$. You can say that $\mathbf{u}$ and $\mathbf{v}$ are antiparallel if $\hat{\mathbf{u}} = -\hat{\mathbf{v}}$. 
:::

## Solving vector equations

By combining addition and scalar multiplication, you can form vector
equations. It is extremely important to be able to solve vector equations. They have many applications in varied field such as geometry, mechanics, multivariable calculus and more. In addition, solving vector equations is one of the key studies of linear mathematics.

One thing to remember from [Guide: Introduction to vectors](introductiontovectors.qmd) is that vectors are only equal if and only if their components are individually equal. That is, if $\mathbf{a} = a_1 \mathbf{i} + a_2 \mathbf{j} + a_3 \mathbf{k}$ and $\mathbf{b} = b_1 \mathbf{i} + b_2 \mathbf{j} + b_3 \mathbf{k}$ are two vectors, then $$\mathbf{a} = \mathbf{b}\quad\textsf{ if and only if }\quad a_1 = b_1,\, a_2 = b_2,\, a_3 = b_3.$$

This means that to solve vector equations, you may have to solve three equations simultaneously! This requires an excellent knowledge of solving simultaneous equations; see [Guide: Solving simultaneous equations] for more.

Solving vector equations is best done when following the lead of examples; here are two. The first of these involves **position vectors**: see [Guide: Introduction to vectors](introductiontovectors.qmd) for more.

<!-- ::: callout-note -->
<!-- ## Solving vector equations -->

<!-- If $\lambda \mathbf{a} + \mu \mathbf{b} = \mathbf{c}$ -->

<!-- Then in $\textbf{i}$,$\textbf{j}$,$\textbf{k}$ notation, -->

<!-- let $\mathbf{a} = a_1\mathbf{i} + a_2\mathbf{j}$,$\mathbf{b} = b_1\mathbf{i} + b_2\mathbf{j}$ -->
<!-- and $\mathbf{c} = c_1\mathbf{i} + c_2\mathbf{j}$. -->

<!-- The equation gives -->

<!-- $\lambda(a_1\mathbf{i} + a_2\mathbf{j} )+ \mu(b_1\mathbf{i} + b_2\mathbf{j}) = c_1\mathbf{i} + c_2\mathbf{j}$ -->

<!-- In column notation, -->

<!-- $\mathbf{a} = \begin{bmatrix}a_1\\a_2\end{bmatrix}$, $\mathbf{b} = \begin{bmatrix}b_1\\b_2\end{bmatrix}$ and -->
<!-- $\mathbf{c} = \begin{bmatrix}c_1\\c_2\end{bmatrix}$. -->

<!-- The equation gives -->
<!-- $\begin{bmatrix}\lambda a_1 + \mu b_1\\ \lambda a_2 + \mu b_2\end{bmatrix} = \begin{bmatrix}c_1\\c_2\end{bmatrix}$ -->

<!-- Both notations give the same simultaneous equations: -->

<!-- $\begin{cases}\lambda a_1 + \mu b_1 = c_1\\\lambda a_2 + \mu b_2 = c_2\end{cases}$ -->
<!-- ::: -->



<!-- This part is the quick examples for simultaneous equations -->

::: {.callout-note appearance="simple"}
## Example 9

If the co-ordinates of the point $B$ are $(-5,-2,-4)$ and
$\overrightarrow{AB} = \begin{bmatrix}1\\1\\-6\end{bmatrix}$, what are the co-ordinates of $A$?

Using knowledge from [Guide: Introduction to vectors](introductiontovectors.qmd), you can say that the position vector of the point $B$ is $$\overrightarrow{OB} = \begin{bmatrix}-5\\-2\\-4\end{bmatrix}$$

If you can find the value of the position vector $\overrightarrow{OA}$, then you can read off the co-ordinates of the point $A$. Using the definition of vector addition, you can write that $$\overrightarrow{OB} = \overrightarrow{OA} + \overrightarrow{AB}$$ and so $\overrightarrow{OA} = \overrightarrow{OB} - \overrightarrow{AB}$. Therefore
$$\overrightarrow{OA} = \overrightarrow{OB} - \overrightarrow{AB}= \begin{bmatrix}-5\\-2\\-4\end{bmatrix} - \begin{bmatrix}1\\1\\-6\end{bmatrix} = \begin{bmatrix}-6\\-3\\2\end{bmatrix}$$
and so the co-ordinates of $A$ are $(-6,-3,2)$.

:::

::: {.callout-note appearance="simple"}
## Example 10

If $\mathbf{u} = 4\mathbf{i} + 3\mathbf{j}$ and $\mathbf{v} = -\mathbf{i} + 2\mathbf{j}$,
how can you express $7\mathbf{i} + 19\mathbf{j}$ in terms of $\mathbf{u}$ and
$\mathbf{v}$?

What you can do here is take the sum of scalar multiples of $\mathbf{u}$ and $\mathbf{v}$ (known as a **linear combination**) and set this vector equal to $7\mathbf{i} + 19 \mathbf{j}$. It is important that you take these two scalars to be potentially different, so give them different names like $\lambda$ ('lambda') and $\mu$ ('mu'). So
$$7\mathbf{i} + 19 \mathbf{j} = \lambda \mathbf{u} + \mu \mathbf{v}$$ Since $\mathbf{u} = 4\mathbf{i} + 3\mathbf{j}$ and $\mathbf{v} = -\mathbf{i} + 2\mathbf{j}$, this becomes $$7\mathbf{i} + 19 \mathbf{j} = (4\lambda \mathbf{i} + 3\lambda\mathbf{j}) + (-\mu\mathbf{i} + 2\mu\mathbf{j})$$ These two vectors are equal if and only if their components are equal. Therefore, this gives two simultaneous equations 
\begin{align*}
7 &= 4\lambda - \mu \tag{\textsf{$\mathbf{i}$ component}}\\
19 &= 3\lambda + 2\mu \tag{\textsf{$\mathbf{j}$ component}}
\end{align*}
Solving these equations (see [Guide: Solving simultaneous equations] for more) gives $\lambda = 3$ and $\mu = 5$, and so $$7\mathbf{i} + 19\mathbf{j} = 3\mathbf{u} + 5\mathbf{v}.$$
:::

<!-- The third of these involves defining straight lines using vectors: see [Guide: Vector equation of a line] for more. -->

# Quick check problems {-}

<!-- add facility for webexercises to work on html -->

::: {.content-visible when-format="html"}
<!-- add facility to check answers at end rather than one at a time -->

::: {.webex-check .webex-box}
1.  If $\mathbf{a} = \begin{bmatrix}0\\-6\\2\end{bmatrix}$, then what is $7\mathbf{a}$?

Answer: $7\mathbf{a}$ is equal to `r fitb(0)`$\mathbf{i}$ +
`r fitb(-42)`$\mathbf{j}$ + `r fitb(14)`$\mathbf{k}$.

2.  If $\mathbf{b} = 2\mathbf{i} + 6\mathbf{k}$ and
    $\mathbf{c} = -5\mathbf{i} + 3\mathbf{j} + 2\mathbf{k}$, then what is
    $\mathbf{c} + 2\mathbf{b}$?

Answer: $\mathbf{c} + 2\mathbf{b}$ = `r fitb(-1)`$\mathbf{i}$ +
`r fitb(-3)`$\mathbf{j}$ + `r fitb(14)`$\mathbf{k}$.

3.  Given that the coordinates $A = \begin{bmatrix}2\\-1\\4\end{bmatrix}$ and
    $B = \begin{bmatrix}3\\-3\\-6\end{bmatrix}$, what is the vector $\overrightarrow{AB}$?

Answer: `r fitb(1)`$\mathbf{i}$ + `r fitb(-2)`$\mathbf{j}$ +
`r fitb(-2)`$\mathbf{k}$.

4.  You are given three statements below. Decide whether they are true or
    false.

(a) If $\overrightarrow{AB} = 2\mathbf{BC}$, the two vectors are perpendicular.
    Answer: `r torf(FALSE)`.
    
(b) If $12\mathbf{a} - 4\mathbf{b} = 8\mathbf{c}$, then $2\mathbf{c} + \mathbf{b} = 3\mathbf{a}$. Answer: `r torf(TRUE)`.

(c) If $\lambda \mathbf{a} + \mu \mathbf{b} = \mathbf{0}$ and $\mathbf{a}$ and
    $\mathbf{b}$ are parallel non-zero vectors, then
    $\lambda = \mu = 0$ is the only solution to this vector equation. Answer: `r torf(FALSE)`.
    
:::

:::

::: {.content-hidden when-format="html"}
1.  If $\mathbf{a} = \begin{bmatrix}0\\-6\\2\end{bmatrix}$, then what is $7\mathbf{a}$?

2.  If $\mathbf{b} = 2\mathbf{i} + 6\mathbf{k}$ and
    $\mathbf{c} = -5\mathbf{i} + 3\mathbf{j} + 2\mathbf{k}$, then what is
    $\mathbf{c} + 2\mathbf{b}$?

3.  Given that the coordinates $A = \begin{bmatrix}2\\-1\\4\end{bmatrix}$ and
    $B = \begin{bmatrix}3\\-3\\-6\end{bmatrix}$, what is the vector $\overrightarrow{AB}$?

4.  You are given three statements below. Decide whether they are true or
    false.

(a) If $\overrightarrow{AB} = 2\mathbf{BC}$, the two vectors are perpendicular.
    
(b) If $12\mathbf{a} - 4\mathbf{b} = 8\mathbf{c}$, then $2\mathbf{c} + \mathbf{b} = 3\mathbf{a}$.

(c) If $\lambda \mathbf{a} + \mu \mathbf{b} = \mathbf{0}$ and $\mathbf{a}$ and $\mathbf{b}$ are parallel non-zero vectors, then $\lambda = \mu = 0$ is the only solution to this vector equation.

:::

# Further reading {-}

[For more questions on the subject, please go to Questions: Vector addition and
scalar multiplication.](../questions/qs-addandsm.qmd)

To explore more about vectors, including when two vectors are perpendicular, please see [Guide: The scalar product](scalarproduct.qmd).

## Version history and licensing {-}

v1.0: initial version created 08/23 by Renee Knapp and Kin Wang Pang as part of a University of St Andrews STEP project.

  - v1.1: edited 05/24 by tdhc. 

[This work is licensed under CC BY-NC-SA 4.0.](https://creativecommons.org/licenses/by-nc-sa/4.0/?ref=chooser-v1)


