---
title: "Solving exponential equations"
author: "Ritwik Anand, Zheng Chen, Zoe Gemmell"
abstract-title: Summary
abstract: This guide applies the laws of indices to solve equations involving powers; a key skill in mathematics and many areas of science.
categories:
  - Solving equations
  - Algebra
image: FiguresPNG/solvingeqsindices-image.png
---

```{r, setup, include = FALSE}
library("webexercises")
```

*It is highly recommended that you read [Guide: Laws of indices](lawsofindices.qmd) before reading this guide. In addition, [Guide: Logarithms](logarithms.qmd) is recommended but not required for some of the material in this guide.*

In [Guide: Laws of indices](lawsofindices.qmd), you learned about the different ways that you can manipulate expressions involving powers (like $x^3$ and $2^{80}$) and $n$th roots (such as $\sqrt[4]{x}$ and $2^{1/80}$). In general mathematical life however, this knowledge will not be enough; you will need to apply these laws of indices to help you solve equations. 

Solving equations involving indices is a key skill in areas whenever exponential growth or decay plays a role: economics, physics (particularly nuclear physics), chemistry, biology, and many more.

Before you get started however, it is worth reiterating the recommendation above:

::: {.callout-important}

**This guide assumes an excellent knowledge of the laws of indices. Please make sure that you have read [Guide: Laws of indices](lawsofindices.qmd) before continuing.** 

The numbering of the laws will follow the numbering in this guide and on [Factsheet: Laws of indices](../factsheets/f-lawsofindices.qmd).

In addition, an initial understanding of logarithms will be required later in the guide. While this understanding is partially explained in this guide, you may want to familiarize yourself with [Guide: Logarithms](logarithms.qmd) before attempting Examples 7, 8, 9, and 10.

:::

# Discussion of techniques

In general, the golden rule of solving equations involving indices is the following:

::: {.callout-tip}

**Make sure both sides are the in the same base before simplifying**. This is because if $a$ is a positive number not equal to $1$ and $a^m = a^n$, then you can immediately say that $m = n$ and solve the equation from there.

:::

However, you may be wondering; why on earth is this true? How can you ignore the base in this case? Or, more pertinently, *what if you can't write the equation in a form where both sides have the same base*?

What you can do in this case is isolate the variable on one side of the equation, and have a constant on the other (see [Guide: Rearranging equations](introtorearrange for more); perhaps it looks like $a^x = b$. From there, you can take **logarithms** to base $a$ of both sides.

Since for all $a > 0$ with $a \neq 1$ and all real numbers $y$: 

$$\quad a^{\log_a(y)} = y\qquad \textsf{ and }\qquad \log_a (a^y) = y$$
it follows that $$\log_a(a^x) = \log_a b$$ implies that $$x = \log_a b$$ solving the equation! What this means is that logarithms undo exponentiation and exponentiation undoes logarithms. 

In particular, this is why $a^m = a^n$ implies that $m = n$. Taking logarithms to base $a$ of both sides of $a^m = a^n$ gives $\log_a a^m = \log_a a^n$; using the above result then yields $m = n$. 

However, please be aware of the following:

::: {.callout-warning}

**You cannot take logarithms of a negative number!** So an expression like $\log_a(-4)$ is **not** defined.

:::

This is particularly pertinent in Example 9 below.

In this guide, logarithms are only used to undo exponentiation to solve equations; there will not be any applications of the laws of logarithms nor the change of base rule. (For more on these, see [Guide: Logarithms](logarithms.qmd).)

# Examples

## Initial examples {-}

::: {.callout-note appearance="simple"}

## Example 1

Solve $x^{\frac{1}{2}}=8$.

You can start squaring both sides of the equation to get $(x^{\frac{1}{2}})^2 = 8^2$. Using Law 3, $(x^{1/2})^2 = x^{2/2} = x$; so then you get the answer $x = 64$. To check if the answer is correct, you can substitute $64$ back into the equation: $64^{\frac{1}{2}} = \sqrt[2]{64}=8$.

:::

::: {.callout-note appearance="simple"}

## Example 2

Solve $x^{-2}=9$.

Using Law 5, $x^{-2} = 9$ can be re-expressed as $\frac{1}{x^2} = 9$. Multiplying both sides by $x^2$ gives you $1=9x^2$.
Then dividing both sides by $9$ gives you $\frac{1}{9}=x^2$. Remembering you can have positive and negative roots, you get $x= \frac{1}{3}$ or $x= -\frac{1}{3}$ as the two solutions to this equation.

:::

::: {.callout-note appearance="simple"}

## Example 3

Solve $3^{4x}=27^{5-x}$.

You can notice here that the two sides of the equation have different bases; so you need to write these in the same base. As $27=3^3$, the equation can be rewritten as: $3^{4x}=(3^3)^{5-x}$. Then using Law 3, you can write $3^{4x}=3^{15-3x}$. Since the bases of both sides are equal, you can say that $4x=15-3x$. Rearranging gives $x= 15/7$.
:::

::: {.callout-note appearance="simple"}

## Example 4

Solve $x^{\frac{5}{3}} + 3x^{\frac{2}{3}} = 10x^{-\frac{1}{3}}$.

If you look at all of the indices in the question, the denominator is $3$ and that is a hint of what you need to multiply by. Multiply by $x^{\frac{1}{3}}$ on both sides of the equation; using Law 1, this gives
\begin{align*}
x^{\frac{5}{3}}\cdot x^{\frac{1}{3}} + 3x^{\frac{2}{3}}\cdot x^{\frac{1}{3}} &= 10x^{-\frac{1}{3}}\cdot x^{\frac{1}{3}}\\
x^{\frac{6}{3}} + 3x^{\frac{3}{3}} &= 10x^0
\end{align*}
Using Law 4, you can further simplify this expression to get $x^2 +3x = 10$, and so $x^2+3x-10=0$. This is a quadratic equation; factorizing this equation gives you $(x+5)(x-2)=0$, then you can get $x=-5$ and $x=2$ as the two possible solutions to this equation.

:::

<!-- ::: {.callout-tip} -->

<!-- When dealing with equations, you may find yourself faced with the following form: -->
<!-- \begin{align*} -->
<!-- \dfrac{1}{a+\sqrt{b}}\end{align*} -->

<!-- In which case you will want to use the **conjugate** of the denominator to *creatively* multiply the fraction by 1. The conjugate of $a+\sqrt{b}$ is $a-\sqrt{b}$, to find this for any espression you change the sign in front of the root. -->

<!-- \begin{align*} -->
<!-- \dfrac{1}{a+\sqrt{b}}\cdot 1&= \dfrac{1}{a+\sqrt{b}}\cdot\dfrac{a-\sqrt{b}}{a-\sqrt{b}}\nonumber \\[0.5em] -->
<!-- &= \dfrac{a-\sqrt{b}}{(a+\sqrt{b})(a-\sqrt{b})}\nonumber \\[0.5em] -->
<!-- &= \dfrac{a-\sqrt{b}}{a^2+a\sqrt{b}-a\sqrt{b}-(\sqrt{b})^2}\nonumber \\[0.5em] -->
<!-- &= \dfrac{a-\sqrt{b}}{a^2-b} -->
<!-- \end{align*} -->

<!-- Now the fraction only has square roots in the numerator, this is better because it can often make expressions you are dealing with more concise. -->

<!-- ::: -->

:::{.callout-note appearance='simple'}
## Example 5

Solve $2^{x+1}\cdot 3^x =72$. 

Here, you will need to condense the left-hand side into a single base. Using Law 1, you can write that $$2^{x+1}\cdot 3^x = 2(2^x\cdot 3^x) = 72.$$ Next, use Law 7 to combine $2^x$ and $3^x$ into a single base;
$$2(2^x\cdot 3^x) = 2((2\cdot 3)^x) = 2\cdot 6^x = 72.$$
Therefore, $6^x = 36$. Since $36 = 6^2$, it follows that $x = 2$. (Or indeed, you could have taken logarithms of both sides to base $6$.)
:::

:::{.callout-note appearance='simple'}
## Example 6

Solve $\sqrt{(6x)^3}=8\sqrt{27}$.

First of all, you can use Law 7 to write $(6x)^3 = 6^3\cdot x^3$. Using Law 10, you can then write the left hand side of this equation as $$\sqrt{(6x)^3} = \sqrt{6^3\cdot x^3} = \sqrt{6^3}\cdot \sqrt{x^3}$$ You can now work on $\sqrt{6^3}$; using Law 7 and Law 10, you can write $$\sqrt{6^3} = \sqrt{2^3\cdot 3^3} = \sqrt{8}\cdot \sqrt{27}.$$ Therefore, the initial equation becomes $$\sqrt{(6x)^3} = \sqrt{8}\cdot \sqrt{27}\cdot\sqrt{x^3}=8\sqrt{27}.$$ Dividing both sides by $\sqrt{8}$ (thereby using Laws 2 and 6) and cancelling the $\sqrt{27}$ gives $$\sqrt{x^3} = \frac{8}{\sqrt{8}} = \frac{8^1}{8^{1/2}} = 8^{1/2} = \sqrt{8}.$$
Squaring both sides to undo the square root gives $x^3 = 8$, and so $x = 2$.

<!-- Here is a rather long example using multiple laws from this guide and the intro to indices guide. -->

<!-- \begin{align*} -->
<!-- \sqrt{(6x)^3}&=8\sqrt{27}\nonumber \\[0.5em] -->
<!-- \sqrt{x^3}\cdot\sqrt{6^3}&=8\sqrt{27}\tag{\,Using Law 7 and Law 10} \\[0.5em] -->
<!-- \sqrt{x^3}\cdot\sqrt{(2\cdot 3)^3}&=8\sqrt{27}\tag{\,Using Law 7} \\[0.5em] -->
<!-- \sqrt{x^3}\cdot\sqrt{2^3}\sqrt{3^3}&=8\sqrt{27}\tag{\,Using Law 10} \\[0.5em] -->
<!-- \end{align*} -->
<!-- to simplify the appearance of the calculation, swap $2^3$ for $8$ -->
<!-- \begin{align*} -->
<!-- \sqrt{x^3}\cdot\sqrt{8}\sqrt{27}&=8\sqrt{27}\nonumber \\[0.5em] -->
<!-- \sqrt{x^3}\cdot\sqrt{8}&=8\tag{\,cancel $\sqrt{27}$} \\[0.5em] -->
<!-- \sqrt{x^3}&=\dfrac{8}{8^{1/2}}\nonumber \\[0.5em] -->
<!-- \sqrt{x^3}&=\sqrt{8}\tag{\,Using Law 2} \\[0.5em] -->
<!-- \end{align*} -->
<!-- Finally, switch back to $2^3$ -->
<!-- \begin{align*} -->
<!-- x^3&=8=2^3 -->
<!-- \end{align*} -->

<!-- So $x=2$ is the final answer. -->

:::

## Examples involving logarithms {-}

::: {.callout-note appearance="simple"}

## Example 7

Solve $e^{3x}=12$.

Taking the logarithm of both sides to base $e$ gives you $\log_e(e^{3x})=\log_e(12)$. Using the definition of logarithms, you can express the equation as $3x = \ln(12)$. Rearranging the equation gives you $x=\dfrac{\ln(12)}{3}$ and this is your final answer.
:::

::: {.callout-tip}

Although $e$ here was treated as some constant, it is actually a very important constant called *Euler's number*.

In addition, there is a special name for $\log_e(x)$; this is the **natural logarithm** of $x$, often written $\ln(x)$.

To see more about Euler's number $e$ and natural logarithms, please read [Guide: Logarithms](logarithms.qmd).

:::

::: {.callout-note appearance="simple"}

## Example 8

Given the equation $6^x = 3^{x + 1}$, solve for $x$.

First of all, you can notice that as $6$ is not a power of $3$ (or vice versa) getting these in the same base is difficult. What you can do instead is use the laws of indices to get an expression of the form $a^x = b$ and then take logarithms. Using Law 1, you can write that $$6^x = 3^x\cdot 3^1 = 3(3^x)$$ Dividing both sides by $3^x$ and using Law 8 gives $$\left(\frac{6^x}{3^x}\right) = \left(\frac{6}{3}\right)^x = 3$$ and so you are left with $2^x = 3$. Taking logarithms of both sides to base $2$ gives $x = \log_2(3)$; and this is your final answer!

<!-- First, you can take the logarithm of both sides of the equation with base $a > 1$, $$\log_a(3^x) = \log_a(7^{x+1})$$ -->

<!-- Next, using Law 3, you can bring the powers of the arguments outside of the logarithm as follows, $$x\log_a(3) = (x+1)\log_a(7)$$ -->

<!-- After that, expand the right side of the equation to obtain $$x\log_a(3) = x\log_a(7) + \log_a(7)$$ -->

<!-- Subtracting $x\log_a(7)$ from both sides of the equation gives you $$x\log_a(3) - x\log_a(7) = \log_a(7)$$ From which you can pull a factor of $x$ out on the left, giving you $$x \cdot (\log_a(3) - \log_a(7)) = \log_a(7)$$ -->

<!-- Finally, dividing both sides by $(\log_a(3) - \log_a(7))$, you conclude that $$x = \frac{\log_a(7)}{\log_a(3) - \log_a(7)}$$ -->

:::

::: {.callout-note appearance="simple"}

## Example 9

Given the equation $5^{2x} + 7(5^x) - 30 = 0$, you are asked to solve for $x$.

Start by letting $y = 5^x$. Then, you can rewrite the equation given as $(5^x)^2 + 7(5^x) - 30 = 0$ using Law 3, which is the same as writing $$y^2 +7y - 30 = 0.$$

Recognizing that this is a quadratic equation (see [Guide: Introduction to quadratic equations](introtoquadratics.qmd) for more), you can use the quadratic formula or otherwise to show that $$y = -10 \quad \textsf{or} \quad y = 3.$$

As $y = 5^x$, this means that $5^x = -10$ or $5^x = 3$. By taking the logarithm of both sides to base $5$, you can show that $$x = \log_5(-10) \quad \textsf{or} \quad x = \log_5(3).$$  Remember from above that the logarithm of a negative number is not defined, so $x = \log_5(3)$ is the only viable solution.

:::

The final example uses many of the laws of indices!

::: {.callout-note appearance="simple"}

## Example 10

Solve $3^{3x} = 5^{x-4}$.

This example is similar to Example 8, only with a few extra steps. Once again, as $3$ is not a power of $5$ or vice versa, the strategy is to write the equation in the form $a^x = b$ and then take logarithms of both sides. 

First of all, use Law 1 to write $5^{x-4} = 5^x\cdot 5^{-4}$ and Law 3 to write $3^{3x} = (3^3)^x$. Since $3^3 = 27$, the equation becomes $$27^x = 5^x\cdot 5^{-4}$$ Dividing both sides by $5^x$ gives $$\frac{27^x}{5^x} = 5^{-4}$$ Using Law 8 and Law 5, you can write $$\left(\frac{27}{5}\right)^x = \frac{1}{5^4} = \frac{1}{625}$$ Taking logarithms to base $27/5$ on both sides gives $x = \log_{27/5}(1/625)$, which is your final answer.

:::

# Quick check problems {-}

::: {.content-visible when-format="html"}

::: {.webex-check .webex-box data-topic="SEE1"}

*If your answer is not a whole number, you should enter your answers as fractions $a/b$ and **not** decimals.*

1. Solve $3x^3\cdot 5 = 405$ for $x$.

Answer: $x$ is `r fitb("3")`

2. Solve $(9x-1)^{1/3}=4$ for $x$.

Answer: $x$ is `r fitb("65/9")`

3. Solve $x^{3/2}=\dfrac{125}{27}$ for $x$.

Answer: $x$ is `r fitb("25/9")`


:::

:::

::: {.content-hidden when-format="html"}

1. Solve $3x^3\cdot 5 = 405$ for $x$.

2. Solve $(9x-1)^{1/3}=4$ for $x$.

3. Solve $x^{3/2}=\dfrac{125}{27}$ for $x$.

:::

# Further reading {-}

For more questions on the subject, please go to [Questions: Solving exponential equations](../questions/qs-solvingeqsindices.qmd).

## Version history and licensing {-}

v1.0: initial version created 08/23 by Ritwik Anand, Zheng Chen, and Zoë Gemmell as part of a University of St Andrews STEP project.

  - v1.1: edited 04/24 by tdhc.
  
[This work is licensed under CC BY-NC-SA 4.0.](https://creativecommons.org/licenses/by-nc-sa/4.0/?ref=chooser-v1)
  

